bedrock.WeakestPrecondition: CPS more to generate fewer existentials

bedrock2/src/WeakestPrecondition.v
@@ -6,34 +6,42 @@ Section WeakestPrecondition.
   Context {p : unique! Semantics.parameters}.
   Context (rely guarantee : trace -> Prop) (progress : trace -> trace -> Prop).
 
-  Definition get (l : locals) (x : varname) (v : word) : Prop :=
-    map.get l x = Some v.
+  Definition literal v post : Prop :=
+    bind_ex_Some v <- word_of_Z v; post v.
+  Definition get (l : locals) (x : varname) (post : word -> Prop) : Prop :=
+    bind_ex_Some v <- map.get l x; post v.
+  Definition load s m a (post : _ -> Prop) : Prop :=
+    bind_ex_Some v <- load s m a; post v.
+  Definition store sz m a v post :=
+    bind_ex_Some m <- store sz m a v; post m.
 
   Section WithMemAndLocals.
     Context (m : mem) (l : locals).
-    Fixpoint expr (e : Syntax.expr) (v : word) : Prop :=
+    Fixpoint expr (e : Syntax.expr) (post : word -> Prop) : Prop :=
       match e with
-      | expr.literal v' => word_of_Z v' = Some v
-      | expr.var x => get l x v
+      | expr.literal v =>
+        literal v post
+      | expr.var x =>
+        get l x post
       | expr.op op e1 e2 =>
-        bind_ex v1 <- expr e1;
-        bind_ex v2 <- expr e2;
-        interp_binop op v1 v2 = v
+        expr e1 (fun v1 =>
+        expr e2 (fun v2 =>
+        post (interp_binop op v1 v2)))
       | expr.load s e =>
-        bind_ex a <- expr e;
-        load s m a = Some v
+        expr e (fun a =>
+        load s m a post)
     end.
   End WithMemAndLocals.
 
   Section WithF.
-    Context {A B} (f: A -> B -> Prop).
-    Fixpoint list_map (xs : list A) (ys : list B) {struct xs} : Prop :=
+    Context {A B} (f: A -> (B -> Prop) -> Prop).
+    Fixpoint list_map (xs : list A) (post : list B -> Prop) {struct xs} : Prop :=
       match xs with
-      | nil => ys = nil
+      | nil => post nil
       | cons x xs' =>
-        bind_ex y <- f x;
-          exists ys', ys = cons y ys' /\
-                      list_map xs' ys'
+        f x (fun y =>
+        list_map xs' (fun ys' =>
+        post (cons y ys')))
       end.
   End WithF.
 
@@ -44,18 +52,18 @@ Section WeakestPrecondition.
       match c with
       | cmd.skip => post t m l
       | cmd.set x ev =>
-        bind_ex v <- expr m l ev;
+        expr m l ev (fun v =>
         bind_eq l <- map.put l x v;
-        post t m l
+        post t m l)
       | cmd.store sz ea ev =>
-        bind_ex a <- expr m l ea;
-        bind_ex v <- expr m l ev;
-        bind_ex_Some m <- store sz m a v;
-        post t m l
+        expr m l ea (fun a =>
+        expr m l ev (fun v =>
+        store sz m a v (fun m =>
+        post t m l)))
       | cmd.cond br ct cf =>
-        bind_ex v <- expr m l br; (* path-blasting... :( *)
+        expr m l br (fun v => (* path-blasting... :( *)
         (word_test v = true  -> cmd ct t m l post) /\
-        (word_test v = false -> cmd cf t m l post)
+        (word_test v = false -> cmd cf t m l post))
       | cmd.seq c1 c2 =>
         cmd c1 t m l (fun t m l => cmd c2 t m l post)
       | cmd.while e c =>
@@ -63,29 +71,29 @@ Section WeakestPrecondition.
         Coq.Init.Wf.well_founded lt /\
         (exists v, inv v t m l) /\
         (forall v t m l, inv v t m l ->
-          exists b, expr m l e b /\
+          expr m l e (fun b =>
           (word_test b = true -> cmd c t m l (fun t' m l =>
             exists v', inv v' t' m l /\ (progress t' t \/ lt v' v))) /\
-          (word_test b = false -> post t m l))
+          (word_test b = false -> post t m l)))
       | cmd.call binds fname arges =>
-        bind_ex args <- list_map (expr m l) arges;
+        list_map (expr m l) arges (fun args =>
         call fname t m args (fun t m rets =>
           bind_ex_Some l <- map.putmany binds rets l;
-          post t m l)
+          post t m l))
       | cmd.interact binds action arges =>
-        bind_ex args <- list_map (expr m l) arges;
+        list_map (expr m l) arges (fun args =>
         let output := (m, action, args) in
         forall m rets (t := cons (output, (m, rets)) t),
           guarantee t /\
-          (rely t -> (bind_ex_Some l <- map.putmany binds rets l; post t m l))
+          (rely t -> (bind_ex_Some l <- map.putmany binds rets l; post t m l)))
       end.
   End WithFunctions.
 
   Definition func call '(innames, outnames, c) (t : trace) (m : mem) (args : list word) (post : trace -> mem -> list word -> Prop) :=
       bind_ex_Some l <- map.putmany innames args map.empty;
       cmd call c t m l (fun t m l =>
-        bind_ex rets <- list_map (get l) outnames;
-        post t m rets).
+        list_map (get l) outnames (fun rets =>
+        post t m rets)).
           
   Fixpoint call (functions : list (funname * (list varname * list varname * cmd.cmd)))
                 (fname : funname) (t : trace) (m : mem) (args : list word)
